\documentclass{article}
\usepackage[tc]{titlepic}
\usepackage{xcolor}
\usepackage{graphicx}
\usepackage{tipa}
\usepackage{pagecolor,lipsum}
\usepackage{amsmath}
\usepackage{amsfonts}
\usepackage{amssymb}
\usepackage{amsthm}
\usepackage{centernot}
\usepackage{xcolor}
\usepackage{fullpage}
\usepackage{listings}
 
\begin{document}

\begin{proof}
How to derive  $y^2 = x'^3 + Ax' + B$ from $y^2 = x^3 + bx^2 + cx + d$ \\
We use following trick similar to \textbf{Completing the square} in quadratic polynomial\\
\noindent
\begin{equation}
\begin{aligned}
 (x+ \frac{b}{3})^3 &=  x^3 + 3x^2 \frac{b}{3} + 3x (\frac{b}{3})^{2} + (\frac{b}{3})^{3} \\
 (x+ \frac{b}{3})^3 &=  x^3 + bx^2 + 3x (\frac{b}{3})^{2} + (\frac{b}{3})^{3}  \\
 (x+ \frac{b}{3})^3 - [3x (\frac{b}{3})^{2} + (\frac{b}{3})^{3}] &=  x^3 + bx^2 + [3x (\frac{b}{3})^{2} + (\frac{b}{3})^{3}] - [3x (\frac{b}{3})^{2} + (\frac{b}{3})^{3}] \\
 (x+ \frac{b}{3})^3 &=  x^3 + 3x^2 \frac{b}{3} + 3x (\frac{b}{3})^{2} + (\frac{b}{3})^{3} \\ 
 (x+ \frac{b}{3})^3 &=  x^3 + bx^2 + 3x (\frac{b}{3})^{2} + (\frac{b}{3})^{3} \\ 
 (x+ \frac{b}{3})^3 - [3x (\frac{b}{3})^{2} + (\frac{b}{3})^{3}] &=  x^3 + bx^2 + [3x (\frac{b}{3})^{2} + (\frac{b}{3})^{3}] - [3x (\frac{b}{3})^{2} + (\frac{b}{3})^{3}] \\ 
 (x+ \frac{b}{3})^3 - [3x (\frac{b}{3})^{2} + (\frac{b}{3})^{3}] + cx + d &=  x^3 + bx^2 + [3x (\frac{b}{3})^{2} + (\frac{b}{3})^{3}] - [3x (\frac{b}{3})^{2} + (\frac{b}{3})^{3}] + cx + d \\ 
 (x+ \frac{b}{3})^3 - 3x (\frac{b}{3})^{2} - (\frac{b}{3})^{3} + cx + d &=  x^3 + bx^2 + [3x (\frac{b}{3})^{2} + (\frac{b}{3})^{3}] - [3x (\frac{b}{3})^{2} + (\frac{b}{3})^{3}] + cx + d \\ 
 (x+\frac{b}{3})^{3} - [3(\frac{b}{3})^{2} - c]x - (\frac{b}{3})^{3} + d &= x^3 + bx^2 + cx + d  \\ 
\mbox{Let }  x + \frac{b}{3} = x' \mbox{ or } x = x' - \frac{b}{3} \\
 x'^{3} - [3(\frac{b}{3})^{2} - c](x' - \frac{b}{3}) + d - (\frac{b}{3})^3 &= x^3 + bx^2 + cx + d \\
 x'^{3} - [3(\frac{b}{3})^{2} - c]x' + [3(\frac{b}{3})^{2} - c]\frac{b}{3} + d &= x^3 + bx^2 + cx + d  \\
 x'^{3} - [3(\frac{b}{3})^{2} - c]x' + 3(\frac{b}{3})^{3} - \frac{b}{3}c + d &= x^3 + bx^2 + cx + d \\
 x'^{3} +[c-3(\frac{b}{3})^2]x' + 3(\frac{b}{3})^{3} - \frac{b}{3}c + d &= x^3 + bx^2 + cx + d  \\
 \therefore A = [c-3(\frac{b}{3})^2] \quad B =  3(\frac{b}{3})^{3} - \frac{b}{3}c + d \\ 
\end{aligned}
\end{equation} 
\end{proof}

\end{document}

